commit

Projects/IO/Defs.lean
@@ -16,14 +16,40 @@ def ioBit (b : Bit) : ProgM Bit := do
   | [] => .lift # .inl b
   | b₀ :: bs => set bs; pure b₀
 
+@[class]
+structure ProgM.WF {α : Type} (m : ProgM α) : Prop where
+  inr ⦃xs zs r⦄ : m.run xs = .inr (r, zs) → zs <:+ xs ∧ ∀ ⦃ys⦄,
+    m.run (xs ++ ys) = .inr (r, zs ++ ys)
+  inl ⦃xs b⦄ : m.run xs = .inl b → ∀ ⦃ys zs r⦄,
+    m.run (xs ++ ys) = .inr (r, zs) → zs <:+ ys ∧ zs ≠ ys
+
 def ProgM.toProg (m : ProgM Unit) : Prog where
   run bs := match m.run bs with
   | .inl b => b
   | .inr _ => 0
 
-@[class]
-structure ProgM.WF {α : Type} (prog : ProgM α) : Prop where
-  inr {xs zs r} : prog.run xs = .inr (r, zs) → zs <:+ xs ∧ ∀ ⦃ys⦄,
-    prog.run (xs ++ ys) = .inr (r, zs ++ ys)
-  inl {xs ys b} : prog.run xs = .inl b → ∀ ⦃r zs⦄,
-    prog.run (xs ++ ys) = .inr (r, zs) → zs <:+ ys ∧ zs ≠ ys
+def Prog.toProgM (p : Prog) : ProgM Unit := do
+  let bs ← get
+  .lift # .inl # p.run bs
+
+def readBit : ProgM Bit := do
+  ioBit 0
+
+def writeBit (b : Bit) : ProgM Unit := do
+  _ ← ioBit b
+
+def readBitsUntil (p : List Bit → Bool) : ProgM (List Bit) := do
+  let bs ← get
+  match bs.inits.find? p with
+  | some bs₁ =>
+    .set # bs.drop bs₁.length
+    pure bs₁
+  | none => .lift # .inl 0
+
+def readNat : ProgM ℕ := do
+  let bs ← readBitsUntil (0 ∈ ·)
+  pure # bs.length - 1
+
+def writeNat (n : ℕ) : ProgM Unit := do
+  replicateM_ n (writeBit 1)
+  writeBit 0
