Projects/IO/Basic.lean
@@ -1,5 +1,42 @@
 import Projects.IO.Defs
 
+namespace List
+
+variable {α β γ : Type*}
+variable {xs ys zs : List α}
+
+-- #check 0 #exit
+
+end List
+
+section monad
+
+variable {α β γ : Type}
+variable {M : Type → Type} [hM₁ : Monad M] [hM₂ : LawfulMonad M]
+
+omit hM₂ in @[simp]
+theorem sequence_nil : sequence ([] : List (M α)) = pure [] := rfl
+
+-- @[simp]
+-- theorem sequence_cons {m : M α} {ms} :
+-- sequence (m :: ms) = m >>= λ x => sequence ms >>= λ xs => pure (x :: xs) := by
+--   nth_rw 1 [sequence]
+--   simp [traverse, List.traverse]
+
+-- #check 0 #exit
+
+end monad
+
+section MonadState
+
+variable {α β γ : Type}
+variable {σ : Type} {M : Type → Type}
+variable [hσ : MonadState σ M] [hM : Monad M]
+
+-- #check 0 #exit
+
+end MonadState
+
 namespace VerifiedIO
 
 variable {α β γ : Type}
@@ -7,3 +44,150 @@ variable {α β γ : Type}
 @[instance, simp]
 theorem ProgM.wf_pure {x : α} : (pure x : ProgM α).WF := by
   constructor <;> simp
+
+@[instance]
+theorem ProgM.wf_bind {m : ProgM α} {f : α → ProgM β}
+[H₁ : m.WF] [H₂ : ∀ x, (f x).WF] : (m >>= f).WF := by
+  constructor
+  · intro xs zs r h₁;
+    simp at h₁
+    obtain ⟨x, bs, h₁, h₂⟩ := h₁
+    replace H₁ := H₁.1 h₁
+    replace H₂ := (H₂ x).1 h₂
+    obtain ⟨h₃, h₄⟩ := H₁
+    obtain ⟨h₅, h₆⟩ := H₂
+    use h₅.trans h₃
+    intro ys
+    simp [h₄, h₆]
+  · intro xs b h₁ ys zs r h₂
+    simp at h₁ h₂
+    obtain ⟨x, bs, h₂, h₃⟩ := h₂
+    rcases h₁ with h₁ | ⟨y, bs', h₄, h₅⟩
+    · obtain ⟨h₅, h₆⟩ := H₁.2 h₁ h₂
+      obtain ⟨h₇, h₈⟩ := (H₂ x).1 h₃
+      use h₇.trans h₅
+      rintro rfl
+      apply h₆; clear h₆
+      exact List.suffix_antisymm h₅ h₇
+    · obtain ⟨h₆, h₇⟩ := H₁.1 h₄
+      simp [h₇] at h₂; clear h₇
+      rcases h₂ with ⟨rfl, rfl⟩
+      exact (H₂ y).2 h₅ h₃
+
+@[instance]
+theorem ProgM.wf_fmap {m : ProgM α} {f : α → β} [H₁ : m.WF] : (f <$> m).WF :=
+  inferInstanceAs(WF # m >>= λ x => pure (f x))
+
+example : ¬(gets List.length : ProgM _).WF := by
+  rintro ⟨h₁, -⟩; specialize @h₁ [] [] 0 (by rfl)
+  replace h₁ := @h₁.2 [0]; revert h₁; simp
+
+@[instance, simp]
+theorem ProgM.wf_ioBit {b} : (ioBit b).WF := by
+  constructor
+  · intro xs zs r h₁
+    simp [ioBit] at h₁
+    split at h₁ <;> cases h₁
+    nm bs b₁
+    simp
+    intro ys
+    rfl
+  · intro xs b₁ h₁ ys zs r h₂
+    simp [ioBit] at h₁ h₂
+    split at h₂; grind
+    nm bs₀ b₂ bs h₃
+    cases h₂
+    split at h₁
+    · nm bs'
+      simp at h₃
+      subst h₃
+      cases h₁
+      simp
+    nm bs' b₃ bs₁
+    simp at h₃
+    rcases h₃ with ⟨rfl, rfl⟩
+    simp at h₁
+
+@[instance, simp]
+theorem Prog.wf_toProgM {p : Prog} : p.toProgM.WF := by
+  constructor <;> simp [toProgM]
+
+@[simp]
+theorem toProg_toProgM {p : Prog} : p.toProgM.toProg = p := by
+  ext; simp [ProgM.toProg, Prog.toProgM]; simp [bind, Sum.bind]
+
+theorem toProgM_toProg {m : ProgM Unit}
+(h : ∀ bs, ∃ b, m.run bs = .inl b) : m.toProg.toProgM = m := by
+  ext; simp [ProgM.toProg, Prog.toProgM]; simp [bind, Sum.bind]
+  nm bs; choose b h₁ using h bs; simp [h₁]
+
+@[simp] theorem run_ioBit_nil {b} : (ioBit b).run [] = .inl b := rfl
+@[simp] theorem run_ioBit_cons {b b₁ bs} : (ioBit b).run (b₁ :: bs) = .inr (b₁, bs) := rfl
+@[simp] theorem run_readBit_nil : readBit.run [] = .inl 0 := rfl
+@[simp] theorem run_readBit_cons {b bs} : readBit.run (b :: bs) = .inr (b, bs) := rfl
+@[simp] theorem run_writeBit_nil {b} : (writeBit b).run [] = .inl b := rfl
+@[simp] theorem run_writeBit_cons {b b₁ bs} : (writeBit b).run (b₁ :: bs) = .inr ((), bs) := rfl
+
+@[instance, simp]
+theorem ProgM.wf_readBit : readBit.WF := by
+  simp [readBit]
+
+@[instance, simp]
+theorem ProgM.wf_writeBit {b} : (writeBit b).WF := by
+  unfold writeBit; infer_instance
+
+@[instance, simp]
+theorem ProgM.wf_readBitsUntil {p} : (readBitsUntil p).WF := by
+  unfold readBitsUntil; simp; constructor
+  · intro xs zs r h
+    simp at h
+    split at h <;> simp at h
+    nm x bs₁ h₁; clear x
+    rcases h with ⟨rfl, rfl⟩
+    use by simp
+    intro ys
+    simp [h₁]
+    rw [List.drop_append]
+    simp [Nat.sub_eq_zero_iff_le]
+    left
+    replace h₁ := List.mem_of_find?_eq_some h₁
+    simp at h₁
+    grind
+  · intro xs b h₁ ys zs r h₂
+    simp at h₁ h₂
+    split at h₁ <;> simp at h₁
+    nm x h₁; clear x
+    subst h₁
+    simp [h₁] at h₂
+    simp at h₁
+    split at h₂ <;> simp at h₂
+    nm x bs h₃; clear x
+    rcases h₂ with ⟨rfl, rfl⟩
+    rw [List.drop_append]
+    simp
+    have h₂ := h₃
+    replace h₃ := List.mem_of_find?_eq_some h₃
+    simp at h₃
+    have h₄ := List.mem_of_mem_tail h₃
+    simp at h₄
+    obtain ⟨bs, ⟨zs, rfl⟩, rfl⟩ := h₄
+    simp
+    replace h₂ := List.find?_some h₂
+    grind
+
+-- theorem ProgM.wf_sequence {ms : List (ProgM α)} (h : ∀ m ∈ ms, m.WF) : (sequence ms).WF := by
+--   induction ms
+--   ·
+--     simp
+--   nm m ms ih
+--   simp
+
+-- #check 0 #exit
+
+@[instance, simp]
+theorem ProgM.wf_readNat : readNat.WF := by
+  unfold readNat; infer_instance
+
+-- @[instance, simp]
+-- theorem ProgM.writeNat {n} : (writeNat n).WF := by
+--   unfold VerifiedIO.writeNat
