Projects/Util/Basic.lean
@@ -24,7 +24,7 @@ import Projects.Util.Algebra
 import Projects.Util.Complex
 import Projects.Util.Quotient
 import Projects.Util.Multiset
-import Projects.Util.ListBool
+import Projects.Util.BoolList
 import Projects.Util.BoolArray
 import Projects.Util.SetTheory
 import Projects.Util.ByteArray
