Projects/Util/BoolList.lean
@@ -1,0 +1,241 @@
+import Projects.Util.Finset
+
+namespace List
+
+@[simp]
+def incBoolList' (xs : List Bool) (c : Bool) : List Bool :=
+  match xs with
+  | [] => []
+  | x :: xs => (!(x == c)) :: incBoolList' xs (x && c)
+
+def incBoolList (xs : List Bool) : List Bool :=
+  incBoolList' xs true
+
+@[simp]
+def decideBoolList' (p : List Bool → Bool) (xs : List Bool) (n : ℕ) : Bool :=
+  bif !p xs then false else match n with
+  | 0 => true
+  | n + 1 => decideBoolList' p xs.incBoolList n
+
+def decideBoolList (p : List Bool → Bool) (n : ℕ) : Bool :=
+  decideBoolList' p (List.replicate n false) (2 ^ n)
+
+@[simp]
+def BoolListFinset' (xs : List Bool) (n : ℕ) : Finset (List Bool) :=
+  insert xs # match n with
+  | 0 => ∅
+  | n + 1 => BoolListFinset' xs.incBoolList n
+
+def BoolListFinset (n : ℕ) : Finset (List Bool) :=
+  BoolListFinset' (List.replicate n false) (2 ^ n)
+
+-----
+
+@[simp]
+theorem length_incBoolList' {xs : List Bool} {c} : (xs.incBoolList' c).length = xs.length := by
+  induction xs generalizing c; rfl; nm x xs ih; simp [ih]
+
+@[simp]
+theorem length_incBoolList {xs : List Bool} : xs.incBoolList.length = xs.length :=
+  length_incBoolList'
+
+theorem decideBoolList_of {p : List Bool → Prop} [hp : DecidablePred p] {n : ℕ}
+(h : ∀ (xs : List Bool), xs.length = n → p xs) : decideBoolList p n := by
+  unfold decideBoolList
+  generalize h₁ : replicate n false = xs
+  replace h₁ : xs.length = n; simp [←h₁]
+  generalize 2 ^ n = k
+  induction k generalizing xs <;> simp
+  · exact h _ h₁
+  nm k hk
+  use h _ h₁
+  rw [hk]
+  simpa
+
+@[simp]
+theorem incBoolList_nil : [].incBoolList = [] := rfl
+
+@[simp]
+theorem decideBoolList_zero {p : List Bool → Prop} [hp : DecidablePred p] :
+decideBoolList p 0 = decide (p []) := by
+  simp [decideBoolList]
+
+@[simp]
+theorem BoolListFinset_zero : BoolListFinset 0 = {[]} := rfl
+
+theorem of_mem_BoolListFinset {xs n} (h : xs ∈ BoolListFinset n) : xs.length = n := by
+  unfold BoolListFinset at h
+  generalize 2 ^ n = k at h
+  generalize h₁ : replicate n false = zs at h
+  replace h₁ : zs.length = n; simp [←h₁]
+  induction k generalizing zs
+  · simp at h
+    rwa [h]
+  nm k ih
+  simp at h
+  rcases h with rfl | h
+  · exact h₁
+  apply ih _ h
+  simpa
+
+theorem self_mem_BoolListFinset' {xs : List Bool} {n} : xs ∈ xs.BoolListFinset' n := by
+  cases n <;> simp
+
+theorem BoolListFinset'_add {xs : List Bool} {n k} : xs.BoolListFinset' (n + k) =
+xs.BoolListFinset' n ∪ (incBoolList^[n] xs).BoolListFinset' k := by
+  induction n generalizing xs k
+  · simp [self_mem_BoolListFinset']
+  nm n ih; simp [Nat.add_one_add, ih]
+
+theorem mem_BoolListFinset'_iff_exi_iter {zs xs : List Bool} {n} :
+xs ∈ zs.BoolListFinset' n ↔ ∃ k ≤ n, xs = incBoolList^[k] zs := by
+  induction n generalizing zs <;> simp
+  nm n ih
+  rw [ih]; clear ih
+  constructor
+  · rintro (rfl | ⟨k, hk, rfl⟩)
+    · use 0
+      simp
+    use k + 1
+    simp [hk]
+  · rintro ⟨k, hk, rfl⟩
+    cases k <;> simp
+    nm k; right
+    simp at hk
+    use k
+
+theorem incBoolList'_prefix_of_prefix {xs ys : List Bool} {c}
+(h : xs <+: ys) : xs.incBoolList' c <+: ys.incBoolList' c := by
+  induction xs generalizing ys c <;> simp
+  nm x xs ih
+  cases ys
+  · simp at h
+  nm y ys
+  simp at h
+  rcases h with ⟨rfl, h⟩
+  simp [ih h]
+
+theorem incBoolList_prefix_of_prefix {xs ys : List Bool}
+(h : xs <+: ys) : xs.incBoolList <+: ys.incBoolList :=
+  incBoolList'_prefix_of_prefix h
+
+theorem iter_incBoolList_prefix_of_prefix {xs ys : List Bool} {k}
+(h : xs <+: ys) : incBoolList^[k] xs <+: incBoolList^[k] ys := by
+  induction k generalizing xs ys
+  · simpa
+  nm k ih
+  rw [Function.iterate_succ']
+  exact incBoolList_prefix_of_prefix # ih h
+
+@[simp]
+theorem incBoolList'_false {xs : List Bool} : xs.incBoolList' false = xs := by
+  induction xs <;> simp_all
+
+@[simp]
+theorem incBoolList_false_cons {xs : List Bool} :
+(false :: xs).incBoolList = true :: xs := by
+  simp [incBoolList]
+
+@[simp]
+theorem incBoolList_true_cons {xs : List Bool} :
+(true :: xs).incBoolList = false :: xs.incBoolList := by
+  simp [incBoolList]
+
+@[simp]
+theorem incBoolList_incBoolList_cons {x : Bool} {xs : List Bool} :
+(x :: xs).incBoolList.incBoolList = x :: xs.incBoolList := by
+  cases x <;> simp
+
+@[simp]
+theorem iter_incBoolList_cons_mul_two {x : Bool} {xs : List Bool} {k} :
+incBoolList^[k * 2] (x :: xs) = x :: incBoolList^[k] xs := by
+  induction k generalizing xs
+  · simp
+  nm k ih
+  simp_rw [Nat.succ_mul]
+  simp [ih]
+
+@[simp]
+theorem iter_incBoolList_nil {k} : incBoolList^[k] [] = [] := by
+  induction k <;> simp_all
+
+@[simp]
+theorem iter_incBoolList_two_pow {xs : List Bool} {k} :
+incBoolList^[2 ^ k] xs = xs.take k ++ (xs.drop k).incBoolList := by
+  induction k generalizing xs
+  · simp
+  nm n ih
+  cases xs; simp
+  nm x xs
+  simp_rw [Nat.pow_succ, iter_incBoolList_cons_mul_two, take_succ_cons, drop_succ_cons]
+  simp [ih]
+
+theorem mem_BoolListFinset_of {xs n} (h : xs.length = n) : xs ∈ BoolListFinset n := by
+  rw [BoolListFinset, mem_BoolListFinset'_iff_exi_iter]
+  induction xs generalizing n
+  · simp at h; simp [←h, Nat.le_one_iff]
+  nm x xs ih
+  simp at h
+  cases n <;> simp at h; nm n
+  specialize ih h
+  choose k hk ih using ih
+  rw [List.replicate_succ]
+  generalize h₁ : replicate n false = zs at ih ⊢
+  replace h₁ : zs.length = n; simp [←h₁]
+  cases x
+  ·
+    use k * 2, by omega
+    simpa
+  ·
+    rw [le_iff_eq_or_lt] at hk
+    rcases hk with rfl | hk
+    · rw [iter_incBoolList_two_pow] at ih
+      rw [drop_eq_nil_of_le # by omega] at ih
+      simp at ih
+      rw [take_eq_self_of_le # by omega] at ih
+      subst ih
+      use 1, Nat.one_le_two_pow
+      simp
+    use k * 2 + 1, by omega
+    simpa
+
+theorem mem_BoolListFinset_iff_length_eq {xs n} : xs ∈ BoolListFinset n ↔ xs.length = n :=
+  ⟨of_mem_BoolListFinset, mem_BoolListFinset_of⟩
+
+theorem mem_BoolListFinset_iff_exi_iter {xs : List Bool} {n} :
+xs ∈ BoolListFinset n ↔ ∃ k ≤ (2 ^ n), xs = incBoolList^[k] (List.replicate n false) :=
+  mem_BoolListFinset'_iff_exi_iter
+
+theorem decideBoolList_iff_forall_mem_BoolListFinset {p : List Bool → Prop} [hp : DecidablePred p]
+{n : ℕ} : decideBoolList p n ↔ ∀ xs, xs ∈ BoolListFinset n → p xs := by
+  simp [mem_BoolListFinset_iff_exi_iter]
+  unfold decideBoolList
+  generalize replicate n false = zs at ⊢
+  generalize 2 ^ n = m at ⊢
+  induction m generalizing zs
+  · simp
+  nm m ih
+  simp
+  rw [ih]; clear ih
+  constructor
+  · rintro ⟨h₁, h₂⟩ xs k hk rfl
+    cases k; simpa; nm k
+    simp at hk
+    exact h₂ _ _ hk rfl
+  · intro h
+    use h zs 0 (by simp) rfl
+    intro xs k hk
+    exact @h xs (k + 1) (by omega)
+
+theorem of_decideBoolList {p : List Bool → Prop} [hp : DecidablePred p] {xs : List Bool} {n : ℕ}
+(hn : xs.length = n) (h : decideBoolList p n) : p xs := by
+  simp [decideBoolList_iff_forall_mem_BoolListFinset, mem_BoolListFinset_iff_length_eq] at h
+  exact h _ hn
+
+theorem decideBoolList_iff {p : List Bool → Prop} [hp : DecidablePred p] {n : ℕ} :
+decideBoolList p n ↔ ∀ (xs : List Bool), xs.length = n → p xs :=
+  ⟨λ h₁ _ h₂ => of_decideBoolList h₂ h₁, decideBoolList_of⟩
+
+instance {p : List Bool → Prop} [hp : DecidablePred p] {n : ℕ} :
+Decidable # ∀ (xs : List Bool), xs.length = n → p xs :=
+  decidable_of_bool (decideBoolList p n) decideBoolList_iff
