Projects/Util/Monad.lean
@@ -1,6 +1,18 @@
 import Projects.Util.List
 
 variable {α β γ : Type}
+variable {M : Type → Type} [hM : Monad M]
+
+def sequence_ (ms : List (M α)) : M Unit := do
+  _ ← sequence ms
+
+def replicateM (n : ℕ) (m : M α) : M (List α) := do
+  sequence # .replicate n m
+
+def replicateM_ (n : ℕ) (m : M α) : M Unit := do
+  sequence_ # .replicate n m
+
+-----
 
 @[simp]
 theorem Id_pure : (pure : α → Id α) = (λ a => a) := rfl
@@ -10,9 +22,8 @@ theorem Id_bind {m : Id α} {f : α → Id β} : m >>= f = f m := rfl
 
 section MonadState
 
-variable {α β γ : Type}
-variable {σ : Type} {M : Type → Type}
-variable [hσ : MonadState σ M] [hM : Monad M]
+variable {σ : Type}
+variable [hσ : MonadState σ M]
 
 @[always_inline, inline]
 def gets (f : σ → α) : M α := do pure # f (←get)
@@ -22,7 +33,13 @@ m₂.run (m₁.run x).2 = (do (λ _ => ()) <$> m₁; m₂).run x := rfl
 
 omit hσ in @[simp]
 theorem run_gets {f : σ → α} :
-StateT.run (@gets α σ (StateT σ M) _ _ f) =
+StateT.run (@gets α (StateT σ M) _ σ _ f) =
 StateT.run (@get _ (StateT σ M) _ >>= λ x => pure (f x)) := rfl
+
+omit hσ in @[simp]
+theorem run_set {s : σ} : StateT.run (@set σ (StateT σ M) _ s) = λ _ => pure ((), s) := rfl
+
+omit hσ in @[simp]
+theorem run_set' {s : σ} : StateT.run (StateT.set s : StateT σ M Unit) = λ _ => pure ((), s) := rfl
 
 end MonadState
