Projects/Util/Sum.lean
@@ -6,3 +6,23 @@ variable {α β γ : Type}
 
 @[simp]
 theorem pure_eq {x : β} : (pure x : α ⊕ β) = .inr x := rfl
+
+@[simp]
+theorem bind_eq_inl_iff {m : α ⊕ β} {f : β → α ⊕ γ} {x : α} :
+(m >>= f) = .inl x ↔ m = .inl x ∨ ∃ y, m = .inr y ∧ f y = .inl x := by
+  simp [bind, Sum.bind]; grind
+
+@[simp]
+theorem bind_eq_inr_iff {m : α ⊕ β} {f : β → α ⊕ γ} {x : γ} :
+(m >>= f) = .inr x ↔ ∃ y, m = .inr y ∧ f y = .inr x := by
+  simp [bind, Sum.bind]; grind
+
+@[simp]
+theorem fmap_eq_inl_iff {m : α ⊕ β} {f : β → γ} {x : α} :
+(f <$> m) = .inl x ↔ m = .inl x := by
+  simp [Functor.map, Sum.bind]; grind
+
+@[simp]
+theorem fmap_eq_inr_iff {m : α ⊕ β} {f : β → γ} {x : γ} :
+(f <$> m) = .inr x ↔ ∃ y, m = .inr y ∧ f y = x := by
+  simp [Functor.map, Sum.bind]; grind
